universal_deduction.v
@@ -18,40 +18,42 @@ Section universals.
 
   Variable nd : list form -> form -> Prop.
   Notation "A ⊢ p" := (nd A p) (at level 70).
-  Variable ndH : forall A p, In p A -> A ⊢ p.
 
   Definition up_ctx (A : list form) := map (subst_form (S >> var_term)) A.
   Inductive nd_univ (A : list form) : form -> Prop :=
-    | ndUAgree p : A ⊢ p -> A ⊢U p
     | ndUI p : up_ctx A ⊢ p -> A ⊢U ∀ p
     | ndUE p t : A ⊢ ∀ p -> A ⊢U subst_form (scons t (var_term)) p
   where "A ⊢U p" := (nd_univ A p).
 
-  Variable agree : forall A p, A ⊢U p -> A ⊢ p.
-
+(*   Variable agree : forall A p, A ⊢U p -> A ⊢ p.
+ *)
   Variable weakening : forall A B p, A ⊢ p -> incl A B -> B ⊢ p.
   Lemma weakening_univ A B p : A ⊢U p -> incl A B -> B ⊢U p.
-  Proof. intro. revert B. destruct H; intros B Hinc; [ apply ndUAgree | apply ndUI | apply ndUE ].
-    1,3: now apply (weakening A).
+  Proof. intro. revert B. destruct H; intros B Hinc; [ apply ndUI | now apply ndUE, (weakening A) ].
     -apply (weakening (up_ctx A) (up_ctx B)); [ assumption | unfold up_ctx ]. now apply incl_map.
   Defined.
 
 
-  Variable retract_implicative : included form_implicative form.
-
+(*   Variable retract_implicative : included form_implicative form.
+ *)
   Variable translate : form -> form.
-  Definition translate_univ (p : form_universal form) : form := match p with
-    | All _ q => ¬¬(∀ (translate q))
+  Definition translate_univ (p : form_universal form) : _ := match p with
+    | All _ q => All _ (translate q)
   end.
 
+  Variable translation_inj : forall p, translate (inj p) = inj (translate_univ p).
+  Variable translation_subst : forall q sigma, translate (subst_form sigma q) = subst_form sigma (translate q).
   Variable translation_int : forall A p, A ⊢ p -> (map translate A) ⊢ (translate p).
-  Lemma translation_int_univ A p : A ⊢U p -> (map translate A) ⊢U (translate p).
-  Proof. intro H. apply agree in H. apply translation_int in H. now apply ndUAgree.
-  Defined.
 
-  Variable translation_elim : forall A p, (map translate A) ⊢ (translate p) -> A ⊢ p.
-  Lemma translation_elim_univ A p : (map translate A) ⊢U (translate p) -> A ⊢U p.
-  Proof. intro. now apply ndUAgree, translation_elim, agree.
+  Lemma translation_map A: up_ctx (map translate A) = map translate (up_ctx A).
+  Proof. unfold up_ctx. repeat rewrite map_map. apply map_ext. intro p. symmetry. apply translation_subst.
+  Qed.
+
+  Lemma translation_int_univ A p : A ⊢U p -> (map translate A) ⊢U (translate p).
+  Proof. destruct 1.
+    -rewrite translation_inj. cbn. apply ndUI. rewrite translation_map. now apply translation_int.
+    -rewrite translation_subst. apply ndUE. pose (translation_inj (All _ p)). cbn in e. rewrite <- e.
+     now apply translation_int.
   Defined.
 
 End universals.
